Sections & Instances fixed

Bank_Arrangement.ml
@@ -27,16 +27,16 @@ module BankArrangement (P : BankParams) = struct
 
   let reboot = Bank_Coq.reboot
   let systemName = "Distributed Banking System"
-  let init (n : name) = magic (bank_multi_params.init_handlers (magic n))
+  let init (n : name) = magic (final_multi_params.init_handlers (magic n))
 
   type client_id = Bank_Coq.clientId
   let createClientId () = char_list_of_string (Uuidm.to_string (Uuidm.create `V4))
   let serializeClientId (c : char list) = string_of_char_list c
 
   let handleIO (n : name) (i : input) (s : state) =
-    magic (bank_multi_params.input_handlers (magic n) (magic i) (magic s))
+    magic (final_multi_params.input_handlers (magic n) (magic i) (magic s))
   let handleNet (d : name) (n : name) (m : msg) (s : state) =
-    magic (bank_multi_params.net_handlers (magic d) (magic n) (magic m) (magic s))
+    magic (final_multi_params.net_handlers (magic d) (magic n) (magic m) (magic s))
 
   let deserializeMsg = Bank_Serialization.deserializeMsg
   let serializeMsg = Bank_Serialization.serializeMsg
@@ -52,6 +52,6 @@ module BankArrangement (P : BankParams) = struct
   (* FIXME: Timeouts are arbitrary right now *)
   let setTimeout _ _ = Random.float 0.5
   let handleTimeout (n : name) (s : state) =
-    magic (bank_multi_params.input_handlers
+    magic (final_multi_params.input_handlers
                (magic n) (magic (NetI ([], Timeout))) (magic s))
 end
