Bank.v
@@ -10,7 +10,10 @@ Require String.
 
 Module Import NatDict := FMapList.Make(Nat_as_OT).
 
+Set Bullet Behavior "Strict Subproofs".
+
 Section Bank.
+
   Definition Account := Nat_as_OT.t.
   Definition Account_eq_dec : forall a a' : Account, {a = a'} + {a <> a'}.
     decide equality.
@@ -149,7 +152,7 @@ Section Bank.
 
   Definition ServerIOHandler (ni : NetInput) : ServerStateHandler := nop.
 
-  Instance bank_base_params : BaseParams :=
+  Global Instance bank_base_params : BaseParams :=
   {
     data   := State ;
     input  := NetInput ;
@@ -174,10 +177,10 @@ Section Bank.
 
   Definition NetHandler (dst src : Name) (nm : NetMsg) (s : State) :=
     match (dst , s) with
-    | (Agent  , agent  astate) =>
+    | (Agent, agent  astate) =>
         let '(a,b,c) := runGenHandler_ignore astate (AgentNetHandler nm)
         in (a, agent b, c)
-    | (Server , server sstate) =>
+    | (Server, server sstate) =>
         let '(a,b,c) := runGenHandler_ignore sstate (ServerNetHandler nm)
         in (a, server b, c)
     | _ => runGenHandler_ignore s nop
@@ -185,16 +188,16 @@ Section Bank.
 
   Definition IOHandler (n : Name) (ni : NetInput) (s : State) :=
     match (n , s) with
-    | (Agent  , agent  astate) =>
+    | (Agent, agent astate) =>
         let '(a,b,c) := runGenHandler_ignore astate (AgentIOHandler ni)
         in (a, agent b, c)
-    | (Server , server sstate) =>
+    | (Server, server sstate) =>
         let '(a,b,c) := runGenHandler_ignore sstate (ServerIOHandler ni)
         in (a, server b, c)
     | _ => runGenHandler_ignore s nop
     end.
 
-  Instance bank_multi_params : MultiParams bank_base_params :=
+  Global Instance bank_multi_params : MultiParams bank_base_params :=
   {
     name := Name ;
     name_eq_dec := Name_eq_dec;
@@ -213,197 +216,9 @@ Section Bank.
 
   (* FIXME: X_X *)
   Definition reboot (state : State) : State := state.
-  Instance failure_params : FailureParams _ :=
+  Global Instance bank_failure_params : FailureParams _ :=
   {
     reboot := reboot
   }.
-
-  (* Repeated unfolding of all handler monads *)
-  Ltac bank_handlers_unfold :=
-    repeat (monad_unfold ; unfold NetHandler,
-                                  AgentNetHandler, ServerNetHandler,
-                                  IOHandler,
-                                  AgentIOHandler, ServerIOHandler
-                                  in *).
-
-(* 
-  SAFETY for STATES, no need now
-
-  Definition valid_values (m : ServerState) : Prop := 
-    forall acc v,
-      NatDict.find acc m = Some v ->
-      v >= 0.
-
-  Definition bank_correct (sigma : Name -> State) : Prop :=
-    match (sigma Server) with
-    | agent  _      => False
-    | server sstate => valid_values sstate
-    end.
-
-  Lemma bank_correct_init :
-    bank_correct init_handlers.
-  Proof using.
-    simpl. discriminate.
-  Qed.
-  
-  Definition timeout_case (i : NetInput) (out : list NetOutput) (st : State) (st' : State) (ms : list (Name * NetMsg)) :=
-  match st with
-  | server ss => False
-  | agent _ => exists cid, i = netI cid (Timeout) /\ out = [] /\ ms = []
-  end.
-  
-  Definition create_case (i : NetInput) (out : list NetOutput) (st : State) (st' : State) (ms : list (Name * NetMsg)) :=
-  match st with
-  | server ss => False
-  | agent _ => exists a cid, i = netI cid (Create a) /\ out = [] /\ ms = [(Server, netM cid (req (CreateMsg a)))]
-  end.
-  
-  Definition deposit_case (i : NetInput) (out : list NetOutput) (st : State) (st' : State) (ms : list (Name * NetMsg)) :=
-  match st with
-  | server ss => False
-  | agent _ => exists a v cid, i = netI cid (Deposit a v) /\ out = []  /\ ms = [(Server, netM cid (req (DepositMsg a v)))]
-  end.
-  
-  Definition withdraw_case (i : NetInput) (out : list NetOutput) (st : State) (st' : State) (ms : list (Name * NetMsg)) :=
-  match st with
-  | server ss => False
-  | agent _ => exists a v cid, i = netI cid (Withdraw a v) /\ out = [] /\ ms = [(Server, netM cid (req (WithdrawMsg a v)))]
-  end.
-
-  Definition check_case (i : NetInput) (out : list NetOutput) (st : State) (st' : State) (ms : list (Name * NetMsg)) :=
-  match st with
-  | server ss => False
-  | agent _ => exists a cid, i = netI cid (Check a) /\ out = [] /\ ms = [(Server, netM cid (req (CheckMsg a)))]
-  end.
-
-  Ltac handler_unfold :=
-    repeat (monad_unfold; unfold NetHandler,
-                                 IOHandler,
-                                 ServerNetHandler,
-                                 AgentNetHandler,
-                                 AgentIOHandler,
-                                 ServerIOHandler in .
-  
-  Lemma IOHandler_cases:
-  forall name input state netout state' ms,
-    IOHandler name input state = (netout, state', ms) ->
-    (name = Agent /\ (timeout_case input netout state state' ms \/ create_case input netout state state' ms \/ deposit_case input netout state state' ms \/ withdraw_case input netout state state' ms \/ check_case input netout state state' ms)) \/ (netout = [] /\ state = state' /\ ms = []). 
-  Proof.
-  handler_unfold. intros.
-  repeat break_match;
-  repeat tuple_inversion;
-  [left|left|left|left|left|left|left|right|right|right]; 
-  try intuition.
-  - left. unfold timeout_case. repeat eexists.
-  - right. left. unfold create_case. repeat eexists.
-  - right. right. left. unfold deposit_case. repeat eexists.
-  - right. right. right. left. unfold withdraw_case. repeat eexists.
-  - repeat (try right). unfold check_case. repeat eexists.
-Qed.
-
-  Lemma bank_correct_io_handlers :
-    forall name input sigma st' netout ms,
-      IOHandler name input (sigma name) = (netout, st', ms) ->
-      bank_correct sigma ->
-      bank_correct (update name_eq_dec sigma name st').
-  Proof. 
-  Admitted.
-   
-  Lemma bank_correct_net_handlers :
-    forall p sigma st' out ms,
-      NetHandler (pDst p) (pSrc p) (pBody p) (sigma (pDst p)) = (out, st', ms) ->
-      bank_correct sigma ->
-      bank_correct (update name_eq_dec sigma (pDst p) st').
-  Proof.
-  Admitted.
-  
-  Theorem true_in_reachable_bank_correct :
-  true_in_reachable step_async step_async_init (fun net => bank_correct (nwState net)).
-  Proof.
-  Admitted.*)
-
-
-  (*
-   * Basic lemmas on steps and traces
-   *)
-
-  Lemma step_star_no_trace_no_step :
-    forall net net' trace,
-      step_async_star net net' trace ->
-      trace = [] ->
-      net = net'.
-  Proof using.
-    intros. invc H.
-      (* net = net' *)
-      - reflexivity.
-      (* net -> x' -> net' *)
-      - invc H1 ; invc H5.
-  Qed.
-
-  Lemma trace_well_formed :
-    forall net net' trace,
-      step_async_star net net' trace ->
-      (trace = [] \/ exists trace' n io, trace = trace' ++ [(n, io)]).
-  Proof using.
-    intros.
-    find_apply_lem_hyp refl_trans_1n_n1_trace.
-    invcs H.
-    (* net = net' *)
-    - intuition.
-    (* net -> x' -> net' *)
-    - right. invcs H1.
-      + eauto.
-      + exists (cs ++ [(h, inl inp)]), h, (inr out). apply snoc_assoc.
-  Qed.
-
-  (* [SAFETY]
-   * Trace Correctness : Simulate the trace on an interpreter and prove that
-   *                     we get equivalent behaviour on the distributed system.
-   *)
-
-(*  Definition operate (op : Input) (curr : option Value) :=
-    match op with
-    | Timeout          => (curr, curr)
-    | Create   acc     => (curr, curr)
-    | Deposit  acc val => (curr, curr)
-    | Withdraw acc val => (curr, curr)
-    | Check    acc     => (curr, curr)
-    end.
-
-  Fixpoint interpret (acc : Account) (ops : list Input) (init : option Value) :=
-    match ops with
-    | [] => (init, init)
-    | _  => (init, init)
-    end.
-*)
-
-  Definition trace_values (trace : list (name * (input + list output)))
-                          : list Value :=
-    flat_map (fun n_io => match n_io with
-                          | (Server, _)    => nil
-                          | (Agent, inl _) => nil
-                          | (Agent, inr listO) =>
-                              filterMap (fun o => match o with
-                                                  | netO _ Failed => None
-                                                  | netO _ (Passed _ v) => Some v
-                                                  end)
-                                        listO
-                 end)
-              trace.
-
-
-  (* [SAFETY]
-   * No Negative Value : Over all traces, the returned account value
-   *                     is always non-negative.
-   *)
-  Theorem no_negative_value :
-    forall net trace,
-      step_async_star step_async_init net trace ->
-      forall v, List.In v (trace_values trace) -> v >= 0.
-  Proof using.
-    intros net trace H_network_step_star v H_v_in_trace.
-    unfold trace_values in H_v_in_trace.
-    apply in_flat_map in H_v_in_trace.
-  Admitted.
 
 End Bank.
