Bank_Proofs.v
@@ -1,13 +1,202 @@
 Require Import Bank.
 
-Require Import Verdi.Verdi.
+Require Import
+  Verdi.Verdi
+  Verdi.HandlerMonad.
 
 Set Bullet Behavior "Strict Subproofs".
 
-Local Arguments update {_} {_} _ _ _ _ _ : simpl never.
-
 Section Bank_Proof.
-  Context {bank_base_params  : BaseParams}.
-  Context {bank_multi_params : MultiParams bank_base_params}.
+
+  (*******
+   * Tactics
+   *******)
+
+  (* Repeated unfolding of all handler monads *)
+  Ltac bank_handlers_unfold :=
+    repeat (monad_unfold
+           ; unfold InitState,
+                    NetHandler,
+                    AgentNetHandler, ServerNetHandler,
+                    IOHandler,
+                    AgentIOHandler, ServerIOHandler in *).
+
+  (*******
+   * Basic lemmas on steps and traces
+   *******)
+
+  (* Empty trace => No change in network.
+   * [Converse cannot be proved] *)
+  Lemma step_star_no_trace_no_step :
+    forall net net' trace,
+      step_async_star net net' trace ->
+      trace = [] ->
+      net = net'.
+  Proof using.
+    intros. invc H.
+      (* net = net' *)
+      - reflexivity.
+      (* net -> x' -> net' *)
+      - invc H1 ; invc H5.
+  Qed.
+
+  (* In a well-formed trace,
+   * every node must be present in Nodes. *)
+  Lemma trace_well_formed :
+    forall net trace trace' n io,
+      step_async_star step_async_init net trace ->
+      (trace = [] \/ (trace = trace' ++ [(n, io)] -> (List.In n Nodes))).
+  Proof using.
+    intros. invcs H.
+    (* net = net' *)
+    - intuition.
+    (* net -> x' -> net' *)
+    - right. intuition. apply all_Names_Nodes.
+  Qed.
+
+  Definition trace_values (trace : list (name * (input + list output)))
+                          : list Value :=
+    flat_map (fun n_io => match n_io with
+                          | (Server, _)    => nil
+                          | (Agent, inl _) => nil
+                          | (Agent, inr listO) =>
+                              filterMap (fun o => match o with
+                                                  | netO _ Failed => None
+                                                  | netO _ (Passed _ v) => Some v
+                                                  end)
+                                        listO
+                 end)
+              trace.
+
+  (* [SAFETY]
+   * No Negative Value : Over all traces, the returned account value
+   *                     is always non-negative.
+   *)
+  Theorem no_negative_value :
+    forall net trace,
+      step_async_star step_async_init net trace ->
+      forall v, List.In v (trace_values trace) -> v >= 0.
+  Proof using.
+    intros net trace H_network_step_star v H_v_in_trace.
+    unfold trace_values in H_v_in_trace.
+    apply in_flat_map in H_v_in_trace.
+  Admitted.
+
+(* 
+  SAFETY for STATES, no need now
+
+  Definition valid_values (m : ServerState) : Prop := 
+    forall acc v,
+      NatDict.find acc m = Some v ->
+      v >= 0.
+
+  Definition bank_correct (sigma : Name -> State) : Prop :=
+    match (sigma Server) with
+    | agent  _      => False
+    | server sstate => valid_values sstate
+    end.
+
+  Lemma bank_correct_init :
+    bank_correct init_handlers.
+  Proof using.
+    simpl. discriminate.
+  Qed.
+  
+  Definition timeout_case (i : NetInput) (out : list NetOutput) (st : State) (st' : State) (ms : list (Name * NetMsg)) :=
+  match st with
+  | server ss => False
+  | agent _ => exists cid, i = netI cid (Timeout) /\ out = [] /\ ms = []
+  end.
+  
+  Definition create_case (i : NetInput) (out : list NetOutput) (st : State) (st' : State) (ms : list (Name * NetMsg)) :=
+  match st with
+  | server ss => False
+  | agent _ => exists a cid, i = netI cid (Create a) /\ out = [] /\ ms = [(Server, netM cid (req (CreateMsg a)))]
+  end.
+  
+  Definition deposit_case (i : NetInput) (out : list NetOutput) (st : State) (st' : State) (ms : list (Name * NetMsg)) :=
+  match st with
+  | server ss => False
+  | agent _ => exists a v cid, i = netI cid (Deposit a v) /\ out = []  /\ ms = [(Server, netM cid (req (DepositMsg a v)))]
+  end.
+  
+  Definition withdraw_case (i : NetInput) (out : list NetOutput) (st : State) (st' : State) (ms : list (Name * NetMsg)) :=
+  match st with
+  | server ss => False
+  | agent _ => exists a v cid, i = netI cid (Withdraw a v) /\ out = [] /\ ms = [(Server, netM cid (req (WithdrawMsg a v)))]
+  end.
+
+  Definition check_case (i : NetInput) (out : list NetOutput) (st : State) (st' : State) (ms : list (Name * NetMsg)) :=
+  match st with
+  | server ss => False
+  | agent _ => exists a cid, i = netI cid (Check a) /\ out = [] /\ ms = [(Server, netM cid (req (CheckMsg a)))]
+  end.
+
+  Ltac handler_unfold :=
+    repeat (monad_unfold; unfold NetHandler,
+                                 IOHandler,
+                                 ServerNetHandler,
+                                 AgentNetHandler,
+                                 AgentIOHandler,
+                                 ServerIOHandler in .
+  
+  Lemma IOHandler_cases:
+  forall name input state netout state' ms,
+    IOHandler name input state = (netout, state', ms) ->
+    (name = Agent /\ (timeout_case input netout state state' ms \/ create_case input netout state state' ms \/ deposit_case input netout state state' ms \/ withdraw_case input netout state state' ms \/ check_case input netout state state' ms)) \/ (netout = [] /\ state = state' /\ ms = []). 
+  Proof.
+  handler_unfold. intros.
+  repeat break_match;
+  repeat tuple_inversion;
+  [left|left|left|left|left|left|left|right|right|right]; 
+  try intuition.
+  - left. unfold timeout_case. repeat eexists.
+  - right. left. unfold create_case. repeat eexists.
+  - right. right. left. unfold deposit_case. repeat eexists.
+  - right. right. right. left. unfold withdraw_case. repeat eexists.
+  - repeat (try right). unfold check_case. repeat eexists.
+Qed.
+
+  Lemma bank_correct_io_handlers :
+    forall name input sigma st' netout ms,
+      IOHandler name input (sigma name) = (netout, st', ms) ->
+      bank_correct sigma ->
+      bank_correct (update name_eq_dec sigma name st').
+  Proof. 
+  Admitted.
+   
+  Lemma bank_correct_net_handlers :
+    forall p sigma st' out ms,
+      NetHandler (pDst p) (pSrc p) (pBody p) (sigma (pDst p)) = (out, st', ms) ->
+      bank_correct sigma ->
+      bank_correct (update name_eq_dec sigma (pDst p) st').
+  Proof.
+  Admitted.
+  
+  Theorem true_in_reachable_bank_correct :
+  true_in_reachable step_async step_async_init (fun net => bank_correct (nwState net)).
+  Proof.
+  Admitted.*)
+
+  (* [SAFETY]
+   * Trace Correctness : Simulate the trace on an interpreter and prove that
+   *                     we get equivalent behaviour on the distributed system.
+   *)
+
+(*  Definition operate (op : Input) (curr : option Value) :=
+    match op with
+    | Timeout          => (curr, curr)
+    | Create   acc     => (curr, curr)
+    | Deposit  acc val => (curr, curr)
+    | Withdraw acc val => (curr, curr)
+    | Check    acc     => (curr, curr)
+    end.
+
+  Fixpoint interpret (acc : Account) (ops : list Input) (init : option Value) :=
+    match ops with
+    | [] => (init, init)
+    | _  => (init, init)
+    end.
+*)
 
 End Bank_Proof.
