Bank_SN.v
@@ -1,0 +1,11 @@
+Require Import Bank.
+
+Require Import Verdi.SeqNum.
+
+Set Bullet Behavior "Strict Subproofs".
+
+Section Bank_SN.
+  Definition bank_sn_base_params    := base_params.
+  Definition bank_sn_multi_params   := multi_params.
+  Definition bank_sn_failure_params := bank_failure_params.
+End Bank_SN.
