Bank_SN_Extract.v
@@ -1,6 +1,6 @@
 Require Import Verdi.Verdi.
 
-Require Bank.
+Require Bank_SN.
 
 Require Import
   ExtrOcamlBasic
@@ -14,9 +14,9 @@ Require Import
   Verdi.ExtrOcamlList
   Verdi.ExtrOcamlFin.
 
-Definition final_base_params := Bank.bank_base_params.
-Definition final_multi_params := Bank.bank_multi_params.
-Definition final_failure_params := Bank.bank_failure_params.
+Definition final_base_params := Bank_SN.bank_sn_base_params.
+Definition final_multi_params := Bank_SN.bank_sn_multi_params.
+Definition final_failure_params := Bank_SN.bank_sn_failure_params.
 
 Extraction Language Ocaml.
 Extraction "Bank_Coq.ml" seq final_base_params final_multi_params final_failure_params.
