Makefile
@@ -1,29 +1,55 @@
 OCAML = ocamlbuild -package uuidm -package verdi-runtime -I ml
 
-OCAML_BUILD = $(OCAML) -cflags -w,a
+OCAML_BUILD     = $(OCAML) -cflags -w,a
 OCAML_DBG_BUILD = $(OCAML) -cflags -g
 
-BANK_EXTRACT = Bank.v Bank_Extract.v
-BANK_PROVE = Bank.v Bank_Proofs.v
 
-BANK_OCAML = Bank_Coq.ml
-BANK_PROOF = Bank_Proofs.vo
 
-default: bank.native
+BANK_EXTRACT    = Bank.v Bank_Extract.v
+BANK_PROVE      = Bank.v Bank_Proofs.v
+BANK_SN_EXTRACT = Bank.v Bank_SN.v Bank_SN_Extract.v
+BANK_SN_PROVE   = Bank.v Bank_SN.v Bank_SN_Proofs.v
 
-debug: bank.d.byte
+BANK          = Bank_Extract.vo
+BANK_PROOF    = Bank_Proofs.vo
+BANK_SN       = Bank_SN_Extract.vo
+BANK_SN_PROOF = Bank_SN_Proofs.vo
+
+
+
+default: bank
+
+
+$(BANK): $(BANK_EXTRACT)
+	coqc $(BANK_EXTRACT)
 
 $(BANK_PROOF): $(BANK_PROVE)
 	coqc $(BANK_PROVE)
 
-$(BANK_OCAML): $(BANK_EXTRACT)
-	coqc $(BANK_EXTRACT)
+$(BANK_SN): $(BANK_SN_EXTRACT)
+	coqc $(BANK_SN_EXTRACT)
 
-bank.d.byte: $(BANK_PROOF) $(BANK_OCAML)
-	$(OCAML_DBG_BUILD) Bank.d.byte
+$(BANK_SN_PROOF): $(BANK_SN_PROVE)
+	coqc $(BANK_SN_PROVE)
 
-bank.native: $(BANK_OCAML)
+
+bank: $(BANK)
 	$(OCAML_BUILD) Bank.native
+	mv Bank.native bank
+
+bank-dbg: $(BANK_PROOF) $(BANK)
+	$(OCAML_DBG_BUILD) Bank.d.byte
+	mv Bank.d.byte bank-dbg
+
+bank-sn: $(BANK_SN)
+	$(OCAML_BUILD) Bank.native
+	mv Bank.native bank-sn
+
+bank-sn-dbg: $(BANK_SN_PROOF) $(BANK_SN)
+	$(OCAML_DBG_BUILD) Bank.d.byte
+	mv Bank.d.byte bank-sn-dbg
+
+
 
 clean:
 	$(OCAML_BUILD) -clean
